draft syntax

deps/poulet4/lib/P4automata/Syntax.v
@@ -1,9 +1,21 @@
 Require Import String.
 Require Import HAList.
+Require Poulet4.P4cub.Envn.
+Require Poulet4.P4cub.BigStep.BSUtil.
+Require Poulet4.P4automata.P4automaton.
+Module P4A := P4automaton.
+
+Module Env := Poulet4.P4cub.Envn.Env.
+Module EnvUtil := Poulet4.P4cub.BigStep.BSUtil.EnvUtil.
 
 Inductive hdr_ref: Type :=
 | HRVar (var: string)
 | HRField (hdr: hdr_ref) (field: string).
+
+Inductive expr :=
+| EHdr (h: hdr_ref)
+| ELit (bs: list bool).
+(* todo: binops, ...? *)
 
 Inductive state_name: Type := 
 | SNName (s: string)
@@ -14,17 +26,62 @@ Definition state_ref: Type := state_name + bool.
 Record sel_case: Type :=
   { sc_val: list bool;
     sc_st: state_ref }.
-                        
+
 Inductive transition: Type :=
 | TGoto (state: state_ref)
 | TSel (cond: hdr_ref) (cases: list sel_case) (default: string).
+
+Inductive op :=
+| OpNil
+| OpSeq (s1 s2: op)
+| OpExtract (width: BinNums.positive) (hdr: hdr_ref)
+| OpAsgn (lhs: hdr_ref) (rhs: expr)
+| OpBlock (o: op).
 
 Record state: Type :=
   { st_hdr: hdr_ref;
     st_trans: transition }.
 
-Definition automaton (states: list state_name) := 
-  HAList.t (List.map (fun (s: state_name) => (s, state)) states).
-
 Definition t: Type :=
-  { states: list state_name & automaton states }.
+  Env.t state_name state.
+
+Section Interp.
+  Variable (a: t).
+
+  Definition state_type :=
+    { s: state_name | a s <> None }.
+  
+  Definition store := EnvUtil.epsilon.
+  
+  Definition pre_size (state: state_name) : nat.
+  Admitted.
+
+  Definition size (state: state_type) : nat.
+  Admitted.
+
+  Variable (has_extract: forall s H, 0 < size (exist _ s H)).
+
+  Definition update (state: state_type) (bits: list bool) (st: store) : store.
+  Admitted.
+  
+  Definition transitions (s: state_type) (st: store) : state_type + bool.
+  Admitted.
+
+  Lemma cap: forall s, 0 < size s.
+  Proof.
+    intros.
+    destruct s.
+    apply has_extract.
+  Qed.
+  
+
+  Definition interp (a: t) : P4A.p4automaton :=
+    {| P4A.store := store;
+       P4A.states := state_type;
+       P4A.size := size;
+       P4A.update := update;
+       P4A.transitions := transitions;
+       P4A.cap := cap |}.
+End Interp.
+
+                    
